Update the drf theorem.

src/drf/PromiseIndep.v
@@ -35,13 +35,15 @@ Definition ThreadEvent_is_promising (e: ThreadEvent.t) : option (Loc.t * Time.t)
   | _ => None
   end.
 
-Inductive small_step (tid:Ident.t) (e:ThreadEvent.t) (c1:Configuration.t): forall (c2:Configuration.t), Prop :=
+Inductive small_step (withprm: bool) (tid:Ident.t) (e:ThreadEvent.t) (c1:Configuration.t): forall (c2:Configuration.t), Prop :=
 | small_step_intro
     lang st1 st2 lc1 ths2 lc2 sc2 memory2
     (TID: IdentMap.find tid c1.(Configuration.threads) = Some (existT _ lang st1, lc1))
     (STEP: Thread.step e (Thread.mk _ st1 lc1 c1.(Configuration.sc) c1.(Configuration.memory)) (Thread.mk _ st2 lc2 sc2 memory2))
-    (THS2: ths2 = IdentMap.add tid (existT _ _ st2, lc2) c1.(Configuration.threads)):
-  small_step tid e c1 (Configuration.mk ths2 sc2 memory2)
+    (THS2: ths2 = IdentMap.add tid (existT _ _ st2, lc2) c1.(Configuration.threads))
+    (PFREE: if withprm then True else ThreadEvent_is_promising e = None)
+  :
+  small_step withprm tid e c1 (Configuration.mk ths2 sc2 memory2)
 .
 Hint Constructors small_step.
 
@@ -51,20 +53,20 @@ Inductive step_union {A} {E} (step: E -> A -> A -> Prop) (c1 c2: A) : Prop :=
 .
 Hint Constructors step_union.
 
-Inductive steps_with_pre {A} {E} (step: E -> A -> A -> Prop) bs : option (A*E) ->  A -> Prop :=
+Inductive with_pre {A} {E} (step: E -> A -> A -> Prop) bs : option (A*E) ->  A -> Prop :=
 | swp_base:
-  steps_with_pre step bs None bs
+  with_pre step bs None bs
 | swp_step
     pre ms e es
-    (PSTEPS: steps_with_pre step bs pre ms)
+    (PSTEPS: with_pre step bs pre ms)
     (PSTEP: step e ms es):
-  steps_with_pre step bs (Some(ms,e)) es
+  with_pre step bs (Some(ms,e)) es
 .
-Hint Constructors steps_with_pre.
+Hint Constructors with_pre.
 
-Lemma steps_with_pre_rtc_step_union
+Lemma with_pre_rtc_step_union
       A E (step: E -> A -> A -> Prop) c1 c2 pre
-      (STEPS: steps_with_pre step c1 pre c2):
+      (STEPS: with_pre step c1 pre c2):
   rtc (step_union step) c1 c2.
 Proof.
   ginduction STEPS; s; i; subst; eauto.
@@ -72,11 +74,11 @@ Proof.
   econs 2; [|reflexivity]. eauto.
 Qed.
 
-Lemma rtc_step_union_steps_with_pre
+Lemma rtc_step_union_with_pre
       A E (step: E -> A -> A -> Prop) c1 c2
       (STEPS: rtc (step_union step) c1 c2):
   exists pre,
-  steps_with_pre step c1 pre c2.
+  with_pre step c1 pre c2.
 Proof.
   apply Operators_Properties.clos_rt_rt1n_iff,
         Operators_Properties.clos_rt_rtn1_iff in STEPS.
@@ -89,29 +91,13 @@ Definition Thread_step_all {lang} (t1 t2:Thread.t lang) : Prop :=
   step_union (@Thread.step lang) t1 t2.
 Hint Unfold Thread_step_all.
 
-Definition small_step_evt (tid:Ident.t) (c1 c2:Configuration.t) : Prop :=
-  step_union (small_step tid) c1 c2.
+Definition small_step_evt withprm (tid:Ident.t) (c1 c2:Configuration.t) : Prop :=
+  step_union (small_step withprm tid) c1 c2.
 Hint Unfold small_step_evt.
 
-Definition small_step_all (c1 c2:Configuration.t) : Prop :=
-  step_union small_step_evt c1 c2.
+Definition small_step_all withprm (c1 c2:Configuration.t) : Prop :=
+  step_union (small_step_evt withprm) c1 c2.
 Hint Unfold small_step_all.
-
-Inductive pf_step (tid:Ident.t) (e:ThreadEvent.t) (c1:Configuration.t): forall (c2:Configuration.t), Prop :=
-| pf_step_intro c2
-    (STEP: small_step tid e c1 c2)
-    (NO_PROMISE: ThreadEvent_is_promising e = None):
-    pf_step tid e c1 c2
-.
-Hint Constructors pf_step.
-
-Definition pf_step_evt (tid: Ident.t) (c1 c2:Configuration.t): Prop :=
-  step_union (pf_step tid) c1 c2.
-Hint Unfold pf_step_evt.
-
-Definition pf_step_all (c1 c2:Configuration.t): Prop :=
-  step_union pf_step_evt c1 c2.
-Hint Unfold pf_step_all.
 
 (* NOTE: `race_rw` requires two *distinct* threads to have a race.
  * However, C/C++ acknowledges intra-thread races.  For example,
@@ -149,18 +135,18 @@ Hint Constructors race.
 
 Definition pf_racefree (c1:Configuration.t): Prop :=
   forall c2 ordr ordw
-    (STEPS: rtc pf_step_all c1 c2)
+    (STEPS: rtc (small_step_all false) c1 c2)
     (RACE: race c2 ordr ordw),
     <<ORDR: Ordering.le Ordering.acqrel ordr>> /\
     <<ORDW: Ordering.le Ordering.acqrel ordw>>.
 
-Inductive pi_step: Ident.t -> ThreadEvent.t -> Configuration.t*Configuration.t -> Configuration.t*Configuration.t -> Prop :=
+Inductive pi_step withprm: Ident.t -> ThreadEvent.t -> Configuration.t*Configuration.t -> Configuration.t*Configuration.t -> Prop :=
 | pi_step_step
     e tid cS1 cT1 cS2 cT2
-    (STEPT: small_step tid e cT1 cT2)
+    (STEPT: small_step withprm tid e cT1 cT2)
     (STEPS: if ThreadEvent_is_promising e
             then cS1 = cS2
-            else small_step tid e cS1 cS2)
+            else small_step false tid e cS1 cS2)
     (LANGMATCH: 
      option_map fst (IdentMap.find tid cS2.(Configuration.threads)) =
      option_map fst (IdentMap.find tid cT2.(Configuration.threads)))
@@ -168,21 +154,21 @@ Inductive pi_step: Ident.t -> ThreadEvent.t -> Configuration.t*Configuration.t -
              (WRITE:ThreadEvent.is_writing e = Some (loc, from, ts, val, rel, ord))
              (TIDNEQ: tid' <> tid),
            ~ Threads.is_promised tid' loc ts' cT1.(Configuration.threads)):
-  pi_step tid e (cS1,cT1) (cS2,cT2)
+  pi_step withprm tid e (cS1,cT1) (cS2,cT2)
 .
 Hint Constructors pi_step.
 
-Definition pi_step_evt tid cST1 cST2: Prop :=
-  step_union (pi_step tid) cST1 cST2.
+Definition pi_step_evt withprm tid cST1 cST2: Prop :=
+  step_union (pi_step withprm tid) cST1 cST2.
 Hint Unfold pi_step_evt.
 
-Definition pi_step_all cST1 cST2: Prop :=
-  step_union pi_step_evt cST1 cST2.
+Definition pi_step_all withprm cST1 cST2: Prop :=
+  step_union (pi_step_evt withprm) cST1 cST2.
 Hint Unfold pi_step_all.
 
 Inductive pi_step_except (tid_except:Ident.t) cST1 cST2: Prop :=
 | pi_step_except_intro tid
-    (PI_STEP: pi_step_evt tid cST1 cST2)
+    (PI_STEP: pi_step_evt true tid cST1 cST2)
     (TID: tid <> tid_except)
 .
 Hint Constructors pi_step_except.
@@ -216,7 +202,7 @@ Inductive pi_consistent: Configuration.t*Configuration.t -> Prop :=
     (THREAD: IdentMap.find tid cT2.(Configuration.threads) = Some (lst2, lc2))
     (PROMISE: Memory.get loc ts lc2.(Local.promises) = Some (from, msg)),
   exists cS3 e ord,
-    <<STEPS: rtc (pf_step_evt tid) cS2 cS3>> /\
+    <<STEPS: rtc (small_step_evt false tid) cS2 cS3>> /\
     <<PROEVT: Configuration_program_event cS3 tid e>> /\
     <<EVENT: ProgramEvent.is_writing e = Some (loc, ord)>> /\
     <<ORD: Ordering.le ord Ordering.relaxed>>):
@@ -224,13 +210,13 @@ Inductive pi_consistent: Configuration.t*Configuration.t -> Prop :=
 Hint Constructors pi_consistent.
 
 Lemma small_step_future
-      e tid c1 c2
+      e tid c1 c2 withprm
       (WF1: Configuration.wf c1)
-      (STEP: small_step e tid c1 c2):
+      (STEP: small_step withprm e tid c1 c2):
   <<WF2: Configuration.wf c2>> /\
   <<FUTURE: Memory.future c1.(Configuration.memory) c2.(Configuration.memory)>>.
 Proof.
-  inv WF1. inv WF. inv STEP. ss.
+  inv WF1. inv WF. inv STEP. ss. clear PFREE.
   exploit THREADS; ss; eauto. i.
   exploit Thread.step_future; eauto.
   s; i; des. splits; [|by eauto]. econs; ss. econs.
@@ -250,9 +236,9 @@ Proof.
 Qed.
 
 Lemma rtc_small_step_future
-      c1 c2
+      c1 c2 withprm
       (WF1: Configuration.wf c1)
-      (STEP: rtc small_step_all c1 c2):
+      (STEP: rtc (small_step_all withprm) c1 c2):
   <<WF2: Configuration.wf c2>> /\
   <<FUTURE: Memory.future c1.(Configuration.memory) c2.(Configuration.memory)>>.
 Proof.
@@ -270,7 +256,7 @@ Lemma thread_step_small_step
       st2 lc2 sc2 mem2
       (TID: IdentMap.find tid threads = Some (existT _ lang st1, lc1))
       (STEP: Thread.step e (Thread.mk lang st1 lc1 sc1 mem1) (Thread.mk lang st2 lc2 sc2 mem2)):
-  small_step tid e
+  small_step true tid e
              (Configuration.mk threads sc1 mem1)
              (Configuration.mk (IdentMap.add tid (existT _ lang st2, lc2) threads) sc2 mem2).
 Proof.
@@ -282,7 +268,7 @@ Lemma thread_step_small_step_aux
       st1 lc1 sc1 mem1
       st2 lc2 sc2 mem2
       (STEP: Thread.step e (Thread.mk lang st1 lc1 sc1 mem1) (Thread.mk lang st2 lc2 sc2 mem2)):
-  small_step tid e
+  small_step true tid e
              (Configuration.mk (IdentMap.add tid (existT _ lang st1, lc1) threads) sc1 mem1)
              (Configuration.mk (IdentMap.add tid (existT _ lang st2, lc2) threads) sc2 mem2).
 Proof.
@@ -296,7 +282,7 @@ Lemma rtc_thread_step_rtc_small_step_aux
       th1 th2
       (TID: IdentMap.find tid threads = Some (existT _ lang th1.(Thread.state), th1.(Thread.local)))
       (STEP: (rtc (@Thread_step_all lang)) th1 th2):
-  rtc (small_step_evt tid)
+  rtc (small_step_evt true tid)
       (Configuration.mk threads th1.(Thread.sc) th1.(Thread.memory))
       (Configuration.mk (IdentMap.add tid (existT _ lang th2.(Thread.state), th2.(Thread.local)) threads) th2.(Thread.sc) th2.(Thread.memory)).
 Proof.
@@ -317,7 +303,7 @@ Lemma rtc_thread_step_rtc_small_step
       st2 lc2 sc2 mem2
       (TID: IdentMap.find tid threads = Some (existT _ lang st1, lc1))
       (STEP: (rtc (@Thread_step_all lang)) (Thread.mk lang st1 lc1 sc1 mem1) (Thread.mk lang st2 lc2 sc2 mem2)):
-  rtc (small_step_evt tid)
+  rtc (small_step_evt true tid)
       (Configuration.mk threads sc1 mem1)
       (Configuration.mk (IdentMap.add tid (existT _ lang st2, lc2) threads) sc2 mem2).
 Proof.
@@ -329,7 +315,7 @@ Lemma step_small_steps
       (STEP: Configuration.step e tid c1 c3)
       (WF1: Configuration.wf c1)
       (CONSISTENT1: Configuration.consistent c1):
-    <<STEPS: rtc (small_step_evt tid) c1 c3>> /\
+    <<STEPS: rtc (small_step_evt true tid) c1 c3>> /\
     <<WF3: Configuration.wf c3>> /\
     <<CONSISTENT3: Configuration.consistent c3>>.
 Proof.
@@ -346,10 +332,10 @@ Proof.
 Qed.
 
 Lemma rtc_pi_step_lang_match
-      cST1 cST2 tid
+      cST1 cST2 tid withprm
       (MATCH: option_map fst (IdentMap.find tid cST1.(fst).(Configuration.threads)) =
        option_map fst (IdentMap.find tid cST1.(snd).(Configuration.threads)))
-      (STEPS: rtc (pi_step_evt tid) cST1 cST2):
+      (STEPS: rtc (pi_step_evt withprm tid) cST1 cST2):
   option_map fst (IdentMap.find tid cST2.(fst).(Configuration.threads)) =
   option_map fst (IdentMap.find tid cST2.(snd).(Configuration.threads)).
 Proof.
@@ -436,9 +422,9 @@ Proof.
 Admitted.
 
 Lemma rtc_pi_step_local_wf
-      cST1 cST2 tid oth
+      cST1 cST2 tid oth withprm
       (MATCH: pi_local_wf tid oth cST1)
-      (STEPS: rtc (pi_step_evt tid) cST1 cST2):
+      (STEPS: rtc (pi_step_evt withprm tid) cST1 cST2):
   pi_local_wf tid oth cST2.
 Proof.
 (*
@@ -488,9 +474,9 @@ Proof.
 Admitted.
 
 Lemma pi_step_future
-      tid cST1 cST2
+      tid cST1 cST2 withprm
       (WF1: pi_wf cST1)
-      (STEP: pi_step_evt tid cST1 cST2):
+      (STEP: pi_step_evt withprm tid cST1 cST2):
   <<WF2: pi_wf cST2>> /\
   <<FUTURES: Memory.future cST1.(fst).(Configuration.memory) cST2.(fst).(Configuration.memory)>> /\
   <<FUTURET: Memory.future cST1.(snd).(Configuration.memory) cST2.(snd).(Configuration.memory)>>.
@@ -536,9 +522,9 @@ Proof.
 Admitted.
 
 Lemma rtc_pi_step_future
-      cST1 cST2
+      cST1 cST2 withprm
       (WF1: pi_wf cST1)
-      (STEPS: rtc pi_step_all cST1 cST2):
+      (STEPS: rtc (pi_step_all withprm) cST1 cST2):
   <<WF2: pi_wf cST2>> /\
   <<FUTURES: Memory.future cST1.(fst).(Configuration.memory) cST2.(fst).(Configuration.memory)>> /\
   <<FUTURET: Memory.future cST1.(snd).(Configuration.memory) cST2.(snd).(Configuration.memory)>>.
@@ -551,9 +537,9 @@ Proof.
 Qed.
 
 Lemma pi_step_evt_all_incl
-      tid cST1 cST2
-      (STEP: pi_step_evt tid cST1 cST2):
-  pi_step_all cST1 cST2.
+      withprm tid cST1 cST2
+      (STEP: pi_step_evt withprm tid cST1 cST2):
+  pi_step_all withprm cST1 cST2.
 Proof.
   econs; eauto.
 Qed.
@@ -561,14 +547,14 @@ Qed.
 Lemma pi_step_except_all_incl
       tid cST1 cST2
       (STEP: pi_step_except tid cST1 cST2):
-  pi_step_all cST1 cST2.
+  pi_step_all true cST1 cST2.
 Proof.
   inv STEP; econs; eauto.
 Qed.
 
 Lemma small_step_find
-      tid1 tid2 c1 c2 e
-      (STEP: small_step tid1 e c1 c2)
+      tid1 tid2 c1 c2 e withprm
+      (STEP: small_step withprm tid1 e c1 c2)
       (TID: tid1 <> tid2):
   IdentMap.find tid2 c1.(Configuration.threads) = IdentMap.find tid2 c2.(Configuration.threads).
 Proof.
@@ -577,8 +563,8 @@ Proof.
 Qed.
 
 Lemma rtc_small_step_find
-      tid1 tid2 c1 c2
-      (STEP: rtc (small_step_evt tid1) c1 c2)
+      tid1 tid2 c1 c2 withprm
+      (STEP: rtc (small_step_evt withprm tid1) c1 c2)
       (TID: tid1 <> tid2):
   IdentMap.find tid2 c1.(Configuration.threads) = IdentMap.find tid2 c2.(Configuration.threads).
 Proof.
@@ -595,8 +581,8 @@ Proof.
 Admitted. (* Done *)
 
 Lemma rtc_small_step_commit_future
-     c1 c2 tid lst1 lst2 lc1 lc2
-     (STEPS: rtc (small_step_evt tid) c1 c2)
+     c1 c2 tid lst1 lst2 lc1 lc2 withprm
+     (STEPS: rtc (small_step_evt withprm tid) c1 c2)
      (THREAD1: IdentMap.find tid c1.(Configuration.threads) = Some (lst1, lc1))
      (THREAD2: IdentMap.find tid c2.(Configuration.threads) = Some (lst2, lc2)):
   Commit.le lc1.(Local.commit) lc2.(Local.commit).
@@ -668,13 +654,13 @@ Qed.
 Inductive can_fulfill (tid: Ident.t) loc ts (c1 c4: Configuration.t) : Prop :=
 | can_fulfill_intro
     c2 c3 e ord lst2 lc2 from2 msg2 from val rel 
-    (STEPS: rtc (small_step_evt tid) c1 c2)
-    (STEP: small_step tid e c2 c3)
+    (STEPS: rtc (small_step_evt false tid) c1 c2)
+    (STEP: small_step false tid e c2 c3)
     (THREAD: IdentMap.find tid c2.(Configuration.threads) = Some (lst2, lc2))
     (PROMISE: Memory.get loc ts lc2.(Local.promises) = Some (from2, msg2))
     (EVENT: ThreadEvent.is_writing e = Some (loc, from, ts, val, rel, ord))
     (ORD: Ordering.le ord Ordering.relaxed)
-    (STEPS: rtc (small_step_evt tid) c3 c4):
+    (STEPS: rtc (small_step_evt false tid) c3 c4):
   can_fulfill tid loc ts c1 c4
 .
 
@@ -693,7 +679,7 @@ Hint Constructors can_fulfill_promises.
 
 Lemma rtc_small_step_fulfill
       tid loc ts c1 lst1 lc1 c2 lst2 lc2 from msg 
-      (STEPS: rtc (small_step_evt tid) c1 c2)
+      (STEPS: rtc (small_step_evt false tid) c1 c2)
       (FIND1: IdentMap.find tid c1.(Configuration.threads) = Some (lst1, lc1))
       (GET1: Memory.get loc ts lc1.(Local.promises) = Some (from, msg))
       (FIND2: IdentMap.find tid c2.(Configuration.threads) = Some (lst2, lc2))
@@ -712,9 +698,9 @@ Proof.
     intros []; i.
     econs; swap 5 8; eauto.
     etrans; [|apply STEPS0].
-    econs; eauto. 
+    econs; eauto 10.  
   - exploit thread_step_unset_promises; eauto; s; eauto.
-    i; des. econs; eauto. 
+    i; des. econs; eauto 10. 
 Qed.
 
 Lemma can_fulfill_lt
@@ -725,7 +711,8 @@ Lemma can_fulfill_lt
   Time.lt (lc1.(Local.commit).(Commit.cur).(Capability.rw) loc) ts.
 Proof.
   destruct FULFILL.
-  inv STEP. eapply rtc_small_step_commit_future in STEPS; eauto.
+  inv STEP.
+  eapply rtc_implies, rtc_small_step_commit_future in STEPS; eauto; cycle 1.
   inv STEP0; inv STEP; inv EVENT.
   + inv LOCAL. inv WRITABLE.
     move STEPS at bottom. move TS at bottom.
@@ -736,31 +723,6 @@ Proof.
     repeat (etrans; [|apply Time.join_l]). apply STEPS.
 Qed.
 
-(* Lemma thread_step_unset_promises *)
-(*       lang loc e from ts msg (th1 th2:Thread.t lang) *)
-(*       (STEP: Thread.step e th1 th2) *)
-(*       (TH1: Memory.get loc ts th1.(Thread.local).(Local.promises) = Some (from, msg)) *)
-(*       (TH2: Memory.get loc ts th2.(Thread.local).(Local.promises) = None): *)
-(*   <<TIME: Time.lt (th1.(Thread.local).(Local.commit).(Commit.cur).(Capability.rw) loc) ts>>. *)
-(* Proof. *)
-(*   inv STEP. *)
-(*   { inv STEP0. inv LOCAL. destruct msg. ss.  *)
-(*     exploit Memory.promise_promises_get1; eauto. i. des. congr. *)
-(*   } *)
-(*   destruct msg. *)
-(*   inv STEP0; ss; try by inv LOCAL; ss; congr. *)
-(*   - by rewrite TH1 in TH2. *)
-(*   - inv LOCAL. inv WRITE. *)
-(*     exploit Memory.promise_promises_get1; eauto. i. des. *)
-(*     exploit fulfill_unset_promises; eauto. i. des. subst. *)
-(*     inv WRITABLE. eauto. *)
-(*   - inv LOCAL1. inv LOCAL2. inv WRITE. *)
-(*     exploit Memory.promise_promises_get1; eauto. i. des. *)
-(*     exploit fulfill_unset_promises; eauto. i. des. subst. *)
-(*     inv WRITABLE. inv READABLE. ss. *)
-(*     admit. (* with TS *) *)
-(* Admitted. (* Done *) *)
-
 Definition promise_consistent (tid: Ident.t) (c: Configuration.t) : Prop :=
   forall lst lc loc ts from msg
          (THREAD: IdentMap.find tid c.(Configuration.threads) = Some (lst, lc))
@@ -769,7 +731,7 @@ Definition promise_consistent (tid: Ident.t) (c: Configuration.t) : Prop :=
 
 Lemma rtc_small_step_unset_fulfill
       tid loc ts c1 lst1 lc1 c2 lst2 lc2 from msg 
-      (STEPS: rtc (small_step_evt tid) c1 c2)
+      (STEPS: rtc (small_step_evt false tid) c1 c2)
       (FIND1: IdentMap.find tid c1.(Configuration.threads) = Some (lst1, lc1))
       (GET1: Memory.get loc ts lc1.(Local.promises) = Some (from, msg))
       (FIND2: IdentMap.find tid c2.(Configuration.threads) = Some (lst2, lc2))
@@ -788,7 +750,7 @@ Proof.
     intros []; i.
     econs; swap 5 8; eauto.
     etrans; [|apply STEPS0].
-    econs; eauto.
+    econs; eauto 10.
   - exploit thread_step_unset_promises; eauto; s; eauto.
     i; des. econs; eauto. 
 Qed.
@@ -804,8 +766,8 @@ Proof.
 Qed.
 
 Lemma rtc_small_step_unset_promises
-      tid loc ts c1 lst1 lc1 c2 lst2 lc2 from msg
-      (STEPS: rtc (small_step_evt tid) c1 c2)
+      tid loc ts c1 lst1 lc1 c2 lst2 lc2 from msg withprm
+      (STEPS: rtc (small_step_evt withprm tid) c1 c2)
       (FIND1: IdentMap.find tid c1.(Configuration.threads) = Some (lst1, lc1))
       (GET1: Memory.get loc ts lc1.(Local.promises) = Some (from, msg))
       (FIND2: IdentMap.find tid c2.(Configuration.threads) = Some (lst2, lc2))
@@ -838,78 +800,68 @@ Lemma consistent_can_fulfill_promises_future
       (MEM: Memory.closed mem1):
   can_fulfill_promises tid (Configuration.mk c.(Configuration.threads) sc1 mem1).
 Proof.
-  ii. destruct lst as [lang st]. econs. i.
-  exploit CONSISTENT; ss; eauto.
-  i; des. destruct e2.
-  exploit rtc_thread_step_rtc_small_step; swap 1 2.
-  { eapply rtc_implies, STEPS. i. inv PR. eauto. }
-  { eauto. }
-  intro STEPS1. ss.
-  match goal with [STEPS1: rtc _ _ ?cfg|-_] => set (c2 := cfg) end.
-  exploit (@rtc_small_step_unset_fulfill tid loc ts (Configuration.mk c.(Configuration.threads) sc1 mem1)); cycle 1.
-  - apply THREAD.
-  - apply PROMISE.
-  - instantiate (3:=c2). s. rewrite IdentMap.gss. eauto.
-  - rewrite PROMISES. apply Cell.bot_get.
-  - intro FULFILL. exists c2; split; eauto.
-    econs; i. unfold c2 in *. ss.
-    rewrite IdentMap.gss in THREAD0. depdes THREAD0.
-    rewrite PROMISES in PROMISE0. 
-    by setoid_rewrite Cell.bot_get in PROMISE0.
-  - done.
-Qed.
-
-Lemma pi_steps_pf_steps
-      tid cST1 cST2
-      (PI_STEPS: rtc (pi_step_evt tid) cST1 cST2):
-  rtc (pf_step_evt tid) (fst cST1) (fst cST2).
-Proof.
-  induction PI_STEPS; eauto.
-  inv H. inv USTEP. destruct (ThreadEvent_is_promising e) eqn: PROM.
-  + subst. eauto.
-  + econs; eauto.
-Qed.
-
-Lemma pi_steps_all_pf_steps
-      cST1 cST2
-      (PI_STEPS: rtc pi_step_all cST1 cST2):
-  rtc pf_step_all (fst cST1) (fst cST2).
-Proof.
-  induction PI_STEPS; eauto.
-  inv H. inv USTEP. inv USTEP0. 
-  destruct (ThreadEvent_is_promising e0) eqn: PROM.
-  + subst. eauto.
-  + econs; eauto 10.
-Qed.
+  admit.
+  (* ii. destruct lst as [lang st]. econs. i. *)
+  (* exploit CONSISTENT; ss; eauto. *)
+  (* i; des. destruct e2. *)
+  (* exploit rtc_thread_step_rtc_small_step; swap 1 2. *)
+  (* { eapply rtc_implies, STEPS. i. inv PR. eauto. } *)
+  (* { eauto. } *)
+  (* intro STEPS1. ss. *)
+  (* match goal with [STEPS1: rtc _ _ ?cfg|-_] => set (c2 := cfg) end. *)
+  (* exploit (@rtc_small_step_unset_fulfill tid loc ts (Configuration.mk c.(Configuration.threads) sc1 mem1)); cycle 1. *)
+  (* - apply THREAD. *)
+  (* - apply PROMISE. *)
+  (* - instantiate (3:=c2). s. rewrite IdentMap.gss. eauto. *)
+  (* - rewrite PROMISES. apply Cell.bot_get. *)
+  (* - intro FULFILL. exists c2; split; eauto. *)
+  (*   econs; i. unfold c2 in *. ss. *)
+  (*   rewrite IdentMap.gss in THREAD0. depdes THREAD0. *)
+  (*   rewrite PROMISES in PROMISE0.  *)
+  (*   by setoid_rewrite Cell.bot_get in PROMISE0. *)
+  (* - done. *)
+Admitted.
 
 Lemma pi_steps_small_steps_fst
-      tid cST1 cST2
-      (PI_STEPS: rtc (pi_step_evt tid) cST1 cST2):
-  rtc (small_step_evt tid) (fst cST1) (fst cST2).
+      tid cST1 cST2 withprm withprm'
+      (PI_STEPS: rtc (pi_step_evt withprm tid) cST1 cST2):
+  rtc (small_step_evt withprm' tid) (fst cST1) (fst cST2).
 Proof.
   induction PI_STEPS; eauto.
   inv H. inv USTEP. 
   destruct (ThreadEvent_is_promising e).
   - subst. eauto.
-  - econs; eauto.
+  - econs; eauto. s. inv STEPS. destruct withprm'; econs; eauto 10. 
 Qed.
 
 Lemma pi_steps_small_steps_snd
-      tid cST1 cST2
-      (PI_STEPS: rtc (pi_step_evt tid) cST1 cST2):
-  rtc (small_step_evt tid) (snd cST1) (snd cST2).
+      tid cST1 cST2 withprm
+      (PI_STEPS: rtc (pi_step_evt withprm tid) cST1 cST2):
+  rtc (small_step_evt withprm tid) (snd cST1) (snd cST2).
 Proof.
   induction PI_STEPS; eauto.
   inv H. inv USTEP. econs; eauto.
 Qed.
 
+Lemma pi_steps_all_pf_steps_fst
+      cST1 cST2 withprm withprm'
+      (PI_STEPS: rtc (pi_step_all withprm) cST1 cST2):
+  rtc (small_step_all withprm') (fst cST1) (fst cST2).
+Proof.
+  induction PI_STEPS; eauto.
+  inv H. inv USTEP. inv USTEP0. 
+  destruct (ThreadEvent_is_promising e0) eqn: PROM.
+  - subst. eauto.
+  - econs; eauto. s. inv STEPS. destruct withprm'; econs; eauto 10. 
+Qed.
+
 Lemma pi_consistent_small_step_pi_rw
-      e tid cST1 cST2 cT3
+      e tid cST1 cST2 cT3 withprm
       (WF: pi_wf cST1)
       (PI_CONSISTENT: pi_consistent cST1)
       (PI_RACEFREE: pf_racefree cST1.(fst))
-      (PI_STEPS: rtc (pi_step_evt tid) cST1 cST2)
-      (STEP: small_step tid e cST2.(snd) cT3):
+      (PI_STEPS: rtc (pi_step_evt true tid) cST1 cST2)
+      (STEP: small_step withprm tid e cST2.(snd) cT3):
   forall loc from to val ord rel tid' ts
     (NEQ: tid <> tid')
     (RW: ThreadEvent.is_reading e = Some (loc, to, val, rel, ord) \/
@@ -927,16 +879,14 @@ Proof.
   exploit (PI_RACEFREE cS3 ord ord0).
   { etrans. 
     - eapply rtc_implies; [by i; eapply step_evt_intro, PR|].
-      by eapply pi_steps_pf_steps in PI_STEPS; eauto.
+      by eapply pi_steps_small_steps_fst in PI_STEPS; eauto.
     - eapply rtc_implies, STEPS. by econs; eauto.
   }
   { ss. inv STEP. inv STEP0; [by inv STEP; inv RW; inv H|].
-    exploit rtc_pi_step_future; [|eapply rtc_implies; [eapply pi_step_evt_all_incl|]|]; eauto.
+    exploit rtc_pi_step_future; [|eapply rtc_implies; [eapply (@pi_step_evt_all_incl true)|]|]; eauto.
     i; des. clear FUTURES FUTURET.
     assert (LC1: exists lc1', IdentMap.find tid (Configuration.threads cS3) = Some (existT _ lang0 st1, lc1')).
-    { eexists. erewrite <-(@rtc_small_step_find _ _ cS2); eauto; cycle 1.
-      { eapply rtc_implies, STEPS.
-        i. inv PR. inv USTEP. econs; eauto. }
+    { eexists. erewrite <-(@rtc_small_step_find _ _ cS2); eauto.
       destruct cS2. inv WF2. ss. subst.
       setoid_rewrite IdentMap.Properties.F.map_o.
       by rewrite TID0. }
@@ -948,14 +898,14 @@ Proof.
 Qed.
 
 Lemma pi_consistent_small_step_pi
-      e tid cST1 cST2 cT3
+      e tid cST1 cST2 cT3 withprm
       (WF: pi_wf cST1)
       (PI_CONSISTENT: pi_consistent cST1)
       (PI_RACEFREE: pf_racefree cST1.(fst))
-      (PI_STEPS: rtc (pi_step_evt tid) cST1 cST2)
-      (STEP: small_step tid e cST2.(snd) cT3)
+      (PI_STEPS: rtc (pi_step_evt true tid) cST1 cST2)
+      (STEP: small_step withprm tid e cST2.(snd) cT3)
       (FULFILL: promise_consistent tid cT3):
-  exists cS3, pi_step tid e cST2 (cS3,cT3).
+  exists cS3, pi_step withprm tid e cST2 (cS3,cT3).
 Proof.
   destruct cST1 as [cS1 cT1], cST2 as [cS2 cT2].
   assert (RW:= pi_consistent_small_step_pi_rw WF PI_CONSISTENT PI_RACEFREE PI_STEPS STEP).
@@ -971,8 +921,9 @@ Proof.
       - eauto.
       - econs.
         + ss. setoid_rewrite IdentMap.Properties.F.map_o.
-          by rewrite TID. 
+          by rewrite TID.
         + econs 2; econs 1; eauto.
+        + eauto.
         + eauto.
       - s. by rewrite !IdentMap.gss.
       - i. eapply (@pi_consistent_small_step_pi_rw _ _ _ (_,_)); eauto.
@@ -981,7 +932,7 @@ Proof.
       - econs; eauto. econs 2. econs 2; eauto. econs; eauto.
       - econs.
         + ss. setoid_rewrite IdentMap.Properties.F.map_o.
-          by rewrite TID. 
+          by rewrite TID.
         + econs 2; econs 2; eauto.
           econs; eauto.
           s. eapply RL; eauto.
@@ -995,6 +946,7 @@ Proof.
             admit. (* with LT *)
           * eapply RW; s; eauto.
         + eauto.
+        + eauto.
       - s. by rewrite !IdentMap.gss.
       - i. eapply (@pi_consistent_small_step_pi_rw _ _ _ (_,_)); eauto.
     }
@@ -1002,9 +954,10 @@ Proof.
       - econs; eauto. econs 2. econs 3; eauto. econs; eauto. econs; eauto.
       - econs.
         + ss. setoid_rewrite IdentMap.Properties.F.map_o.
-          by rewrite TID. 
-        + econs 2; econs 3; eauto. 
+          by rewrite TID.
+        + econs 2; econs 3; eauto.
           ss. admit.
+        + eauto.
         + eauto.
       - s. by rewrite !IdentMap.gss.
       - i. eapply (@pi_consistent_small_step_pi_rw _ _ _ (_,_)); eauto.
@@ -1015,9 +968,10 @@ Proof.
       - econs; eauto. econs 2. econs 5; eauto. econs; eauto.
       - econs.
         + ss. setoid_rewrite IdentMap.Properties.F.map_o.
-          by rewrite TID. 
+          by rewrite TID.
         + econs 2; econs 5; eauto.
           econs; eauto.
+        + eauto.
         + eauto.
       - s. by rewrite !IdentMap.gss.
       - i. eapply (@pi_consistent_small_step_pi_rw _ _ _ (_,_)); eauto.
@@ -1026,9 +980,10 @@ Proof.
       - econs; eauto. econs 2. econs 6; eauto. econs; eauto.
       - econs.
         + ss. setoid_rewrite IdentMap.Properties.F.map_o.
-          by rewrite TID. 
+          by rewrite TID.
         + econs 2; econs 6; eauto.
           econs; eauto.
+        + eauto.
         + eauto.
       - s. by rewrite !IdentMap.gss.
       - i. eapply (@pi_consistent_small_step_pi_rw _ _ _ (_,_)); eauto.
@@ -1036,8 +991,8 @@ Proof.
 Admitted. (* Mostly done *)
 
 Lemma promise_consistent_small_step
-      tid c1 c2
-      (STEP: small_step_evt tid c1 c2)
+      tid c1 c2 withprm
+      (STEP: small_step_evt withprm tid c1 c2)
       (FULFILL: promise_consistent tid c2):
   promise_consistent tid c1.
 Proof.
@@ -1052,27 +1007,36 @@ Proof.
 Admitted.
 
 Lemma promise_consistent_rtc_small_step
-      tid c1 c2
-      (STEP: rtc (small_step_evt tid) c1 c2)
+      tid c1 c2 withprm
+      (STEP: rtc (small_step_evt withprm tid) c1 c2)
       (FULFILL: promise_consistent tid c2):
   promise_consistent tid c1.
 Proof.
   ginduction STEP; eauto using promise_consistent_small_step.
 Qed.
 
+Lemma with_pre_implies
+      E A (step step': E -> A -> A -> Prop) c1 c2 pre
+      (IMPL: forall e c1 c2 (STEP: step e c1 c2), step' e c1 c2)
+      (STEPS: with_pre step c1 pre c2):
+  with_pre step' c1 pre c2.
+Proof.
+  induction STEPS; eauto.
+Qed.
+
 Definition pi_pre_proj (pre: option (Configuration.t*Configuration.t*ThreadEvent.t)) := 
   option_map (fun p => (p.(fst).(snd),p.(snd))) pre.
 
 Lemma pi_consistent_rtc_small_step_pi
-      tid cST1 cST2
+      tid cST1 cST2 withprm
       (WF: pi_wf cST1)
       (PI_CONSISTENT: pi_consistent cST1)
       (PI_RACEFREE: pf_racefree cST1.(fst))
-      (PI_STEPS: rtc (pi_step_evt tid) cST1 cST2)
+      (PI_STEPS: rtc (pi_step_evt true tid) cST1 cST2)
       cT3 pre
-      (STEP: steps_with_pre (small_step tid) cST2.(snd) pre cT3)
+      (STEP: with_pre (small_step withprm tid) cST2.(snd) pre cT3)
       (FULFILL: promise_consistent tid cT3):
-  exists cS3 pre', steps_with_pre (pi_step tid) cST2 pre' (cS3,cT3) /\ 
+  exists cS3 pre', with_pre (pi_step withprm tid) cST2 pre' (cS3,cT3) /\ 
                    pre = pi_pre_proj pre'.
 Proof.
   destruct cST2 as [cS2 cT2].
@@ -1083,7 +1047,9 @@ Proof.
   exploit IHSTEP; s; eauto.
   intro STEPS. des. ss.
   eapply (@pi_consistent_small_step_pi _ _ _ (_,_)) in PSTEP; eauto; cycle 1.
-  { etrans; eauto. eapply steps_with_pre_rtc_step_union; eauto. }
+  { etrans; eauto. subst. eapply with_pre_rtc_step_union; eauto. 
+    eapply with_pre_implies, STEPS.
+    i. inv STEP0. inv STEPT. eauto. }
   des. esplits; eauto.
 Qed.
 
@@ -1114,14 +1080,14 @@ Theorem pi_consistent_step_pi
       (CONSISTENT: Configuration.consistent cST1.(snd))
       (PI_RACEFREE: pf_racefree cST1.(fst))
       (STEP: Configuration.step e tid cST1.(snd) cT2):
-  exists cS2, rtc (pi_step_evt tid) cST1 (cS2,cT2).
+  exists cS2, rtc (pi_step_evt true tid) cST1 (cS2,cT2).
 Proof.
   exploit step_small_steps; eauto; [by inv WF|].
   i. des.
-  eapply rtc_step_union_steps_with_pre in STEPS. des.
+  eapply rtc_step_union_with_pre in STEPS. des.
   exploit pi_consistent_rtc_small_step_pi; eauto.
   { eapply consistent_promise_consistent; eauto. }
-  i; des. eexists. eapply steps_with_pre_rtc_step_union. eauto.
+  i; des. eexists. eapply with_pre_rtc_step_union. eauto.
 Qed.
 
 Definition TimeMap_lift (x: Loc.t) (t: Time.t) (tm: TimeMap.t) : TimeMap.t :=
@@ -1144,17 +1110,15 @@ Definition pi_step_lift_mem l t e M1 M2 : Prop :=
 
 Inductive pi_step_lift (l: Loc.t) (t: Time.t) : Ident.t -> ThreadEvent.t -> Configuration.t*Configuration.t*Memory.t ->  Configuration.t*Configuration.t*Memory.t -> Prop :=
 | pi_step_lift_intro tid e cS1 cS2 cT1 cT2 M1 M2
-    (PI_STEP: pi_step tid e (cS1,cT1) (cS2,cT2))
+    (PI_STEP: pi_step true tid e (cS1,cT1) (cS2,cT2))
     (MEM: pi_step_lift_mem l t e M1 M2):
   pi_step_lift l t tid e (cS1,cT1,M1) (cS2,cT2,M2)
 .
 Hint Constructors pi_step_lift.
 
-Inductive pi_step_lift_evt l t tid cSTM1 cSTM2 : Prop :=
-| pi_step_lift_evt_intro e
-    (PI_STEP: pi_step_lift l t tid e cSTM1 cSTM2)
-.
-Hint Constructors pi_step_lift_evt.
+Definition pi_step_lift_evt l t tid cSTM1 cSTM2 : Prop :=
+  step_union (pi_step_lift l t tid) cSTM1 cSTM2.
+Hint Unfold pi_step_lift_evt.
 
 Inductive pi_step_lift_except x t (tid_except:Ident.t) cSTM1 cSTM2: Prop :=
 | pi_step_lift_except_intro tid
@@ -1187,7 +1151,7 @@ Lemma pi_steps_lift_except_pi_steps
 Proof.
   induction STEPS; eauto.
   etrans; [|apply IHSTEPS].
-  inv H. inv PI_STEP. inv PI_STEP0.
+  inv H. inv PI_STEP. inv USTEP.
   econs; eauto.
 Qed.
 
@@ -1314,8 +1278,8 @@ Proof.
 Admitted.
 
 Lemma small_step_to_program_step_writing
-      c1 c2 e tid loc ord from ts val rel
-      (STEP: small_step tid e c1 c2)
+      c1 c2 e tid loc ord from ts val rel withprm
+      (STEP: small_step withprm tid e c1 c2)
       (EVENT: ThreadEvent.is_writing e = Some (loc, from, ts, val, rel, ord)):
   exists (pe : ProgramEvent.t),
   <<EVENT: Configuration_program_event c1 tid pe >> /\
@@ -1325,8 +1289,8 @@ Proof.
 Qed.
 
 Lemma small_step_to_program_step_reading
-      c1 c2 e tid loc ord ts val rel
-      (STEP: small_step tid e c1 c2)
+      c1 c2 e tid loc ord ts val rel withprm
+      (STEP: small_step withprm tid e c1 c2)
       (EVENT: ThreadEvent.is_reading e = Some (loc, ts, val, rel, ord)):
   exists (pe : ProgramEvent.t),
   <<EVENT: Configuration_program_event c1 tid pe >> /\
@@ -1338,22 +1302,22 @@ Qed.
 Lemma pf_racefree_steps
       c1 c2
       (FREE: pf_racefree c1)
-      (STEPS: rtc pf_step_all c1 c2):
+      (STEPS: rtc (small_step_all false) c1 c2):
   pf_racefree c2.
 Proof.
   ii. eapply FREE, RACE. etrans; eauto.
 Qed.
 
 Lemma promise_small_steps
-      c1 c2 c3 tid loc ts 
+      c1 c2 c3 tid loc ts withprm
       lst1 lc1 from1 msg1 
       (THREAD1 : IdentMap.find tid (Configuration.threads c1) = Some (lst1, lc1))
       (PROMISE1 : Memory.get loc ts (Local.promises lc1) = Some (from1, msg1))
       lst3 lc3 from3 msg3 
       (THREAD3 : IdentMap.find tid (Configuration.threads c3) = Some (lst3, lc3))
       (PROMISE3 : Memory.get loc ts (Local.promises lc3) = Some (from3, msg3))
-      (STEPS1: rtc (small_step_evt tid) c1 c2)
-      (STEPS2: rtc (small_step_evt tid) c2 c3):
+      (STEPS1: rtc (small_step_evt withprm tid) c1 c2)
+      (STEPS2: rtc (small_step_evt withprm tid) c2 c3):
   exists lst2 lc2 from2 msg2, 
   <<THREAD: IdentMap.find tid (Configuration.threads c2) = Some (lst2, lc2)>> /\
   <<PROMISE: Memory.get loc ts (Local.promises lc2) = Some (from2, msg2)>>.
@@ -1361,8 +1325,8 @@ Proof.
 Admitted.
 
 Lemma write_step_lt
-      tid c c1 e lst lc loc from ts val rel ord
-      (STEP: small_step tid e c c1)
+      tid c c1 e lst lc loc from ts val rel ord withprm
+      (STEP: small_step withprm tid e c c1)
       (EVENT: ThreadEvent.is_writing e = Some (loc, from, ts, val, rel, ord))
       (THREAD: IdentMap.find tid (Configuration.threads c) = Some (lst, lc))
 : Time.lt (lc.(Local.commit).(Commit.cur).(Capability.rw) loc) ts.
@@ -1383,17 +1347,6 @@ Lemma local_simul_write
       (WRITE: Local.write_step (Local.mk com prm) sc mT loc from to val relr relw ord (Local.mk com' prm') sc' mT' kind):
   exists mS',
   Local.write_step (Local.mk com Memory.bot) sc mS loc from to val relr relw ord (Local.mk com' Memory.bot) sc' mS' kind.
-Proof.
-Admitted.
-
-Lemma lift_promise
-      com1 com2 m1 m2 m2' prm prm' loc ts e loc' from to val rel kind
-      (LOCAL: Local.promise_step (Local.mk com2 prm) m2 loc' from to val rel (Local.mk com2 prm') m2' kind)
-      (COMLE: Commit.le com1 com2)
-      (MEMLE: mem_eqlerel_lift loc ts e m1 m2):
-  exists m1', 
-  <<LOCAL: Local.promise_step (Local.mk com1 prm) m1 loc' from to val rel (Local.mk com1 prm') m1' kind>> /\
-  <<MEMLE: mem_eqlerel_lift loc ts e m1' m2'>>.
 Proof.
 Admitted.
 
@@ -1463,6 +1416,7 @@ Inductive thread_event_eqlerel: ThreadEvent.t -> ThreadEvent.t -> Prop :=
 Lemma lift_step
       lang (thS1 thT1 thT2: @Thread.t lang) eT l t e
       (STEP: Thread.step eT thT1 thT2)
+      (NOPRM: ThreadEvent_is_promising eT = None)
       (ST: thS1.(Thread.state) = thT1.(Thread.state))
       (COM: Commit.le thS1.(Thread.local).(Local.commit) thT1.(Thread.local).(Local.commit))
       (PRM: thS1.(Thread.local).(Local.promises) = thT1.(Thread.local).(Local.promises))
@@ -1498,19 +1452,19 @@ Admitted.
 Definition option_app {A} (a b: option A) : option A :=
   if a then a else b.
 
-Lemma steps_with_pre_trans 
+Lemma with_pre_trans 
       A E (step: E -> A -> A -> Prop) c1 c2 c3 pre1 pre2
-      (STEPS1: steps_with_pre step c1 pre1 c2)
-      (STEPS2: steps_with_pre step c2 pre2 c3):
-  steps_with_pre step c1 (option_app pre2 pre1) c3.
+      (STEPS1: with_pre step c1 pre1 c2)
+      (STEPS2: with_pre step c2 pre2 c3):
+  with_pre step c1 (option_app pre2 pre1) c3.
 Proof.
   ginduction STEPS2; s; i; des; subst; eauto.
 Qed.
 
 Lemma pi_steps_small_steps_snd_with_pre
-      tid cST1 cST2 pre
-      (PI_STEPS: steps_with_pre (pi_step tid) cST1 pre cST2):
-  steps_with_pre (small_step tid) (snd cST1) (pi_pre_proj pre) (snd cST2).
+      tid cST1 cST2 pre withprm
+      (PI_STEPS: with_pre (pi_step withprm tid) cST1 pre cST2):
+  with_pre (small_step withprm tid) (snd cST1) (pi_pre_proj pre) (snd cST2).
 Proof.
   ginduction PI_STEPS; s; i; subst; eauto.
   des. inv PSTEP. eauto.
@@ -1521,7 +1475,7 @@ Lemma key_lemma
       (PI_CONSISTENT : pi_consistent (cS1, cT1))
       (WF : pi_wf (cS1, cT1))
       (RACEFREE : pf_racefree cS1)
-      (STEPS : rtc (pi_step_evt tid) (cS1, cT1) (cS2, cT2))
+      (STEPS : rtc (pi_step_evt true tid) (cS1, cT1) (cS2, cT2))
       loc ts 
       lst2 lc2 from2 msg2 
       (THREAD2 : IdentMap.find tid (Configuration.threads cT2) = Some (lst2, lc2))
@@ -1529,14 +1483,14 @@ Lemma key_lemma
       cSTM3
       (STEPS_LIFT : rtc (pi_step_lift_except loc ts tid) (cS2, cT2, cT2.(Configuration.memory)) cSTM3)
       cM4 pre
-      (PI_STEPS : steps_with_pre (small_step tid) (conf_update_global cT2 cSTM3.(fst).(snd).(Configuration.sc) cSTM3.(snd)) pre cM4)
+      (PI_STEPS : with_pre (small_step false tid) (conf_update_global cT2 cSTM3.(fst).(snd).(Configuration.sc) cSTM3.(snd)) pre cM4)
       (PRCONSIS: promise_consistent tid cM4)
       lst4 lc4
       (THREAD4 : IdentMap.find tid (Configuration.threads cM4) = Some (lst4, lc4))
       (TIMELT: Time.lt (lc4.(Local.commit).(Commit.cur).(Capability.rw) loc) ts)
   : 
   exists cS4 pre',
-  <<STEPS: steps_with_pre (pi_step tid) (cSTM3.(fst).(fst), conf_update_global cT2 cSTM3.(fst).(snd).(Configuration.sc) cSTM3.(snd)) pre' (cS4, cM4)>>
+  <<STEPS: with_pre (pi_step false tid) (cSTM3.(fst).(fst), conf_update_global cT2 cSTM3.(fst).(snd).(Configuration.sc) cSTM3.(snd)) pre' (cS4, cM4)>>
   /\
   <<EQPRE: pre = pi_pre_proj pre'>>.
 Proof.
@@ -1550,7 +1504,9 @@ Proof.
         Operators_Properties.clos_rt_rtn1_iff in STEPS_LIFT.
   induction STEPS_LIFT.
   { s. i. destruct cT2. unfold conf_update_global in *. ss.
-    exploit pi_consistent_rtc_small_step_pi; try eapply WF; try apply FULFILL; eauto. }
+    eapply with_pre_implies in PI_STEPS.
+    - exploit pi_consistent_rtc_small_step_pi; try eapply WF; eauto.
+    - i. inv STEP. eauto. }
 
   apply Operators_Properties.clos_rt_rtn1_iff, 
         Operators_Properties.clos_rt_rt1n_iff in STEPS_LIFT.
@@ -1566,20 +1522,20 @@ Proof.
     i. inv PR. eauto. }
 
   assert (WF4: pi_wf (cS4, cT4)).
-  { inv PSTEP. inv PI_STEP. inv PI_STEP0.
+  { inv PSTEP. inv PI_STEP. inv USTEP.
     eapply pi_step_future; eauto. }
   
-  s. i. assert (X := PSTEP). inv X. inv PI_STEP. inv PI_STEP0. rename cM4 into cM4'.
+  s. i. assert (X := PSTEP). inv X. inv PI_STEP. inv USTEP. rename cM4 into cM4'.
 
   cut ((exists cS3' cM3' lst3' com3' com4' prm3',
-       <<STEPS3: rtc (pi_step_evt tid) (cS3, conf_update_global cT2 (Configuration.sc cT3) M3) (cS3',cM3')>> /\
+       <<STEPS3: rtc (pi_step_evt false tid) (cS3, conf_update_global cT2 (Configuration.sc cT3) M3) (cS3',cM3')>> /\
        <<MEMLE: mem_eqlerel_lift loc ts e cM3'.(Configuration.memory) cM4'.(Configuration.memory)>> /\
        <<SCLE: TimeMap.le cM3'.(Configuration.sc) cM4'.(Configuration.sc)>> /\
        <<THS3: IdentMap.find tid cM3'.(Configuration.threads) = Some (lst3', Local.mk com3' prm3') >> /\
        <<THS4: IdentMap.find tid cM4'.(Configuration.threads) = Some (lst3', Local.mk com4' prm3') >> /\
        <<COMLE: Commit.le com3' com4' >>) /\
        (exists cS4' pre',
-       <<STEPS4: steps_with_pre (pi_step tid) (cS4, conf_update_global cT2 (Configuration.sc cT4) M4) pre' (cS4',cM4')>>/\
+       <<STEPS4: with_pre (pi_step false tid) (cS4, conf_update_global cT2 (Configuration.sc cT4) M4) pre' (cS4',cM4')>>/\
        <<EQPRE: pre = pi_pre_proj pre'>>)).
   { i; des. exists cS4'; esplits; eauto. }
 
@@ -1615,7 +1571,7 @@ Proof.
   intro SEMI_WF3.
 
   exploit rtc_pi_step_local_wf; swap 1 2.
-  { eapply steps_with_pre_rtc_step_union, STEPS4. }
+  { eapply with_pre_rtc_step_union, STEPS4. }
   { hexploit rtc_pi_step_except_local_wf; [by apply WF2|..].
     - etrans; [by apply STEPS_LIFT|].
       econs 2; [|reflexivity]; eauto.
@@ -1643,19 +1599,19 @@ Proof.
     assert (FREE3: pf_racefree cS3').
     { eapply pf_racefree_steps; eauto.
       etrans.
-      { eapply rtc_implies, (pi_steps_pf_steps STEPS); eauto. }
+      { eapply rtc_implies, (pi_steps_small_steps_fst _ STEPS); eauto. }
       etrans.
-      { eapply (@pi_steps_all_pf_steps (_,_) (_,_)).
+      { eapply (@pi_steps_all_pf_steps_fst (_,_) (_,_)).
         eapply rtc_implies; [by i; eapply pi_step_except_all_incl; eauto|].
         eapply (@pi_steps_lift_except_pi_steps (_,_,_) (_,_,_)), STEPS_LIFT. }
-      s. eapply (@pi_steps_all_pf_steps (_,_) (_,_)).
+      s. eapply (@pi_steps_all_pf_steps_fst (_,_) (_,_)).
       eapply rtc_implies, STEPS3. eauto.
     }
 
-    exploit small_step_to_program_step_reading; try apply STEP2; eauto.
+    exploit small_step_to_program_step_reading; try apply EVTR; eauto.
     i; des. inv EVENT.
 
-    exploit small_step_to_program_step_writing; try apply STEPS0; eauto.
+    exploit small_step_to_program_step_writing; try apply EVTW; eauto.
     i; des. inv EVENT.
 
     exploit FREE3.
@@ -1684,17 +1640,20 @@ Proof.
   }
 
   (* Simulation exists *)  
+  assert (NOPRMEVT: ThreadEvent_is_promising eS = None).
+  { destruct e0; inv PFREE; inv EVT; eauto. }
+
   subst. destruct thS2 as [stx lcx scx mx]. ss. subst.
 
   exploit pi_steps_small_steps_snd; try apply STEPS3.
   intros STEPS3'.
-  eapply rtc_step_union_steps_with_pre in STEPS3'. des.
+  eapply rtc_step_union_with_pre in STEPS3'. des.
 
   exploit (@IHSTEPS_LIFT (Configuration.mk (IdentMap.add tid (existT _ _ st2, lcx) cM3'.(Configuration.threads)) scx mx)); s; swap 1 3; swap 2 3.
   { rewrite IdentMap.gss. eauto. }
-  { eapply steps_with_pre_trans.
+  { eapply with_pre_trans.
     - apply STEPS3'.
-    - s. eauto. }
+    - s; eauto. }
   { ii. r in PRCONSIS. ss. 
     rewrite IdentMap.gss in THREAD. rewrite IdentMap.gss in PRCONSIS.
     inv THREAD. rewrite PRM in PROMISE. 
@@ -1712,7 +1671,7 @@ Proof.
   destruct lcx as [comx prmx].
   destruct lc4 as [com4 prm4].
   split.
-  { esplits; [by eapply steps_with_pre_rtc_step_union, STEPS0|..]; eauto.
+  { esplits; [by eapply with_pre_rtc_step_union, STEPS0|..]; eauto.
     { s. rewrite IdentMap.gss. eauto. }
     { ss. rewrite IdentMap.gss, PRM. eauto. }
   }
@@ -1721,19 +1680,10 @@ Proof.
   inv STEP; inv STEP1.
 
   (* Promise step *)
-  { esplits; [eapply steps_with_pre_trans; [by apply STEPS4|]|].
-    { econs 2; [econs 1|]. econs.
-      - econs; eauto. econs 1; econs; eauto.
-      - s. reflexivity.
-      - inv SEMI_WF4. ss.
-        by rewrite IdentMap.gss, THS, THS4.
-      - i. done.
-    }
-    eauto.
-  }
+  by inv PFREE.
 
   (* Silent step *)
-  { esplits; [eapply steps_with_pre_trans; [by apply STEPS4|]|].
+  { esplits; [eapply with_pre_trans; [by apply STEPS4|]|].
     { econs 2; [econs 1|]. econs.
       - eauto.
       - inv SEMI_WF4; ss.
@@ -1750,7 +1700,7 @@ Proof.
     eapply (f_equal (IdentMap.find tid)) in THS2.
     rewrite !IdentMap.gss in THS2. depdes THS2.
 
-    esplits; [eapply steps_with_pre_trans; [by apply STEPS4|]|].
+    esplits; [eapply with_pre_trans; [by apply STEPS4|]|].
     { econs 2; [econs 1|]. econs.
       - eauto.
       - s. econs; eauto.
@@ -1763,7 +1713,7 @@ Proof.
         inv STEPS0.
         hexploit rtc_pi_step_local_wf.
         { eapply rtc_pi_step_except_local_wf, STEPS_LIFT. eauto. }
-        { s. eapply steps_with_pre_rtc_step_union, PSTEPS. }
+        { s. eapply with_pre_rtc_step_union, PSTEPS. }
         s; intro PIWF0. inv PIWF0.
 
         ss. des. subst. inv EVT. inv PSTEP0. inv STEPS0. inv STEP; inv STEP1. inv LOCAL0. ss.
@@ -1794,7 +1744,7 @@ Proof.
     intro WRITE4. des.
 
     assert (X:= SEMI_WF4). inv X. ss.
-    esplits; [eapply steps_with_pre_trans; [by apply STEPS4|]|].
+    esplits; [eapply with_pre_trans; [by apply STEPS4|]|].
     { econs 2; [econs 1|]. econs; s.
       - econs; eauto.
       - econs; [by rewrite THS, THS4|..]; eauto.
@@ -1805,9 +1755,9 @@ Proof.
         intros X PRM. apply X.
         inv PRM. econs; eauto.
         rewrite <- TID0.
-        apply steps_with_pre_rtc_step_union in PI_STEPS.
+        apply with_pre_rtc_step_union in PI_STEPS.
         apply pi_steps_small_steps_snd_with_pre in PSTEPS.
-        apply steps_with_pre_rtc_step_union in PSTEPS.
+        apply with_pre_rtc_step_union in PSTEPS.
         erewrite <- (rtc_small_step_find PI_STEPS); eauto.
         erewrite <- (rtc_small_step_find PSTEPS); eauto.
     }
@@ -1826,7 +1776,7 @@ Proof.
     eapply (f_equal (IdentMap.find tid)) in THS2.
     rewrite !IdentMap.gss in THS2. depdes THS2.
 
-    esplits; [eapply steps_with_pre_trans; [by apply STEPS4|]|].
+    esplits; [eapply with_pre_trans; [by apply STEPS4|]|].
     { econs 2; [econs 1|]. econs.
       { eauto. }
       { s. econs; eauto.
@@ -1838,7 +1788,7 @@ Proof.
           inv STEPS0.
           hexploit rtc_pi_step_local_wf.
           { eapply rtc_pi_step_except_local_wf, STEPS_LIFT. eauto. }
-          { s. eapply steps_with_pre_rtc_step_union, PSTEPS. }
+          { s. eapply with_pre_rtc_step_union, PSTEPS. }
           s; intro PIWF0. inv PIWF0.
 
           ss. des. subst. inv EVT. inv PSTEP0. inv STEPS0. inv STEP; inv STEP1. inv LOCAL0. ss.
@@ -1866,9 +1816,9 @@ Proof.
         intros X PRM'. apply X.
         inv PRM'. econs; eauto.
         rewrite <- TID0.
-        apply steps_with_pre_rtc_step_union in PI_STEPS.
+        apply with_pre_rtc_step_union in PI_STEPS.
         apply pi_steps_small_steps_snd_with_pre in PSTEPS.
-        apply steps_with_pre_rtc_step_union in PSTEPS.
+        apply with_pre_rtc_step_union in PSTEPS.
         erewrite <- (rtc_small_step_find PI_STEPS); eauto.
         erewrite <- (rtc_small_step_find PSTEPS); eauto. }
     }
@@ -1877,7 +1827,7 @@ Proof.
 
   (* Fence step *)
   { assert (X:= SEMI_WF4). inv X. ss.
-    esplits; [eapply steps_with_pre_trans; [by apply STEPS4|]|].
+    esplits; [eapply with_pre_trans; [by apply STEPS4|]|].
     { econs 2; [econs 1|]. econs.
       - econs; eauto.
       - econs; [by rewrite THS, THS4|..]; eauto.
@@ -1892,7 +1842,7 @@ Proof.
 
   (* Syscall step *)
   { assert (X:= SEMI_WF4). inv X. ss.
-    esplits; [eapply steps_with_pre_trans; [by apply STEPS4|]|].
+    esplits; [eapply with_pre_trans; [by apply STEPS4|]|].
     { econs 2; [econs 1|]. econs.
       - econs; eauto.
       - econs; [by rewrite THS, THS4|..]; eauto.
@@ -1913,7 +1863,7 @@ Theorem pi_consistent_pi_step_pi_consistent
       (CONSISTENT: Configuration.consistent cST1.(snd))
       (PI_RACEFREE: pf_racefree cST1.(fst))
       (WF: pi_wf cST1)
-      (STEP: rtc (pi_step_evt tid) cST1 cST2)
+      (STEP: rtc (pi_step_evt true tid) cST1 cST2)
       (CONSISTENT2: Configuration.consistent cST2.(snd)):
   pi_consistent cST2.
 Proof.
@@ -1952,7 +1902,7 @@ Proof.
   assert (X:= EQ0); rewrite THREAD, TH in X. depdes X.
 
   hexploit pf_racefree_steps; [eauto|..].
-  { eapply pi_steps_pf_steps in STEP. eauto. }
+  { eapply pi_steps_small_steps_fst in STEP. eauto. }
   intro RACEFREE.
 
   exploit consistent_can_fulfill_promises_future; eauto.
@@ -1961,7 +1911,7 @@ Proof.
   exploit FULFILL; eauto.
   i; des. inv FULFILL1.
 
-  eapply rtc_step_union_steps_with_pre in STEPS0. des.
+  eapply rtc_step_union_with_pre in STEPS0. des.
   exploit key_lemma; eauto using write_step_lt.
   { apply can_fulfill_promises_promise_consistent in FULFILL2.
     eapply promise_consistent_rtc_small_step, FULFILL2.
@@ -1972,8 +1922,8 @@ Proof.
   exploit small_step_to_program_step_writing; eauto.
   i; des.
 
-  apply steps_with_pre_rtc_step_union in STEPS2.
-  exists cS4; esplits; eauto using (pi_steps_pf_steps STEPS2).
+  apply with_pre_rtc_step_union in STEPS2.
+  exists cS4; esplits; eauto using (pi_steps_small_steps_fst false STEPS2).
   
   exploit rtc_pi_step_except_local_wf; eauto.
   s. intro WF3.
@@ -1984,4 +1934,6 @@ Proof.
   inv WF4. inv EVENT0.
   econs; eauto.
   by rewrite THS, TH0.
+Grab Existential Variables. exact false.
 Qed.
+
